History vlsms (#52)
* History VLSMs and basic results

Co-authored-by: wkolowski <wkolowski@protonmail.com>
Co-authored-by: Karl Palmskog <palmskog@gmail.com>

theories/VLSM/Core/Composition.v
@@ -1537,3 +1537,144 @@ End sec_same_IM_full_projection.
 
 Arguments same_IM_label_rew {_ _ _ _} _ _ : assert.
 Arguments same_IM_state_rew {_ _ _ _} _ _ _ : assert.
+
+Section sec_composite_succ.
+
+Context
+  {message : Type}
+  `{EqDecision index}
+  (IM : index -> VLSM message)
+  `{forall i, HistoryVLSM (IM i)}
+  (Free := free_composite_vlsm IM)
+  (RFree := pre_loaded_with_all_messages_vlsm Free)
+  .
+
+Record CompositeValidTransition l s1 iom s2 oom : Prop :=
+  {
+    cvt_valid : composite_valid IM l (s1, iom);
+    cvt_transition : composite_transition IM l (s1, iom) = (s2, oom)
+  }.
+
+Lemma composite_valid_transition_reachable_iff l s1 iom s2 oom :
+  CompositeValidTransition l s1 iom s2 oom <-> ValidTransition RFree l s1 iom s2 oom.
+Proof. by firstorder. Qed.
+
+Inductive CompositeValidTransitionNext (s1 s2 : composite_state IM) : Prop :=
+| composite_transition_next : forall l iom oom,
+    CompositeValidTransition l s1 iom s2 oom ->
+    CompositeValidTransitionNext s1 s2.
+
+Lemma composite_valid_transition_next :
+  forall l s1 iom s2 oom,
+    CompositeValidTransition l s1 iom s2 oom -> CompositeValidTransitionNext s1 s2.
+Proof. by intros * [Hv Ht]; econstructor. Qed.
+
+Lemma CompositeValidTransitionNext_reachable_iff s1 s2 :
+  CompositeValidTransitionNext s1 s2 <-> ValidTransitionNext RFree s1 s2.
+Proof.
+  by split; intros []; econstructor; apply composite_valid_transition_reachable_iff.
+Qed.
+
+Lemma composite_valid_transition_projection :
+  forall l s1 iom s2 oom,
+    CompositeValidTransition l s1 iom s2 oom ->
+    ValidTransition (IM (projT1 l)) (projT2 l) (s1 (projT1 l)) iom (s2 (projT1 l)) oom /\
+    s2 = state_update IM s1 (projT1 l) (s2 (projT1 l)).
+Proof.
+  intros [i li] * [Hv Ht]; cbn in Ht; destruct (vtransition _ _ _) eqn:Hti.
+  by inversion Ht; subst; cbn; rewrite state_update_eq; repeat split.
+Qed.
+
+Lemma composite_valid_transition_projection_inv :
+  forall i li si1 iom si2 oom,
+    ValidTransition (IM i) li si1 iom si2 oom ->
+    forall s1, s1 i = si1 -> forall s2, s2 = state_update IM s1 i si2 ->
+    CompositeValidTransition (existT i li) s1 iom s2 oom.
+Proof.
+  intros * [Hv Ht] s1 <- s2 ->; split; [done |].
+  by cbn; replace (vtransition _ _ _) with (si2, oom).
+Qed.
+
+Lemma not_CompositeValidTransitionNext_initial :
+  forall s2, composite_initial_state_prop IM s2 ->
+  forall s1, ~ CompositeValidTransitionNext s1 s2.
+Proof.
+  intros s2 Hs2 s1 [* Hs1].
+  apply composite_valid_transition_projection, proj1, valid_transition_next in Hs1; cbn in Hs1.
+  by contradict Hs1; apply not_ValidTransitionNext_initial, Hs2.
+Qed.
+
+Lemma composite_quasi_unique_transition_to_state :
+  forall [s],
+  forall [l1 s1 iom1 oom1], CompositeValidTransition l1 s1 iom1 s oom1 ->
+  forall [l2 s2 iom2 oom2], CompositeValidTransition l2 s2 iom2 s oom2 ->
+  projT1 l1 = projT1 l2 ->
+  l1 = l2 /\ s1 = s2 /\ iom1 = iom2 /\ oom1 = oom2.
+Proof.
+  intros ? [i li1] * Ht1 [_i li2] * Ht2 [=]; subst _i.
+  apply composite_valid_transition_projection in Ht1, Ht2; cbn in Ht1, Ht2.
+  destruct Ht1 as [Ht1 Heq_s], Ht2 as [Ht2 Heqs].
+  rewrite Heq_s in Heqs at 1; clear Heq_s.
+  specialize (unique_transition_to_state Ht1 Ht2) as Heq;
+    destruct_and! Heq; subst; repeat split.
+  extensionality j; destruct (decide (i = j)); [by subst |].
+  apply f_equal with (f := fun s => s j) in Heqs.
+  by rewrite !state_update_neq in Heqs.
+Qed.
+  
+Lemma CompositeValidTransitionNext_reflects_rechability :
+  forall s1 s2, CompositeValidTransitionNext s1 s2 ->
+    valid_state_prop RFree s2 -> valid_state_prop RFree s1.
+Proof.
+  intros s1 s2 Hnext Hs2; revert s1 Hnext.
+  induction Hs2 using valid_state_prop_ind; intros s1 Hnext;
+    [by contradict Hnext; apply not_CompositeValidTransitionNext_initial |].
+  destruct Hnext as [[j lj] iom oom Hnext].
+  destruct l as [i li].
+  destruct (decide (i = j)).
+  - subst; apply input_valid_transition_forget_input in Ht as Hvt.
+    apply composite_valid_transition_reachable_iff in Hvt.
+    specialize (composite_quasi_unique_transition_to_state Hnext Hvt eq_refl) as Heq.
+    destruct_and! Heq; subst.
+    by eapply input_valid_transition_origin.
+  - apply input_valid_transition_forget_input in Ht as Hti.
+    apply composite_valid_transition_reachable_iff,
+      composite_valid_transition_projection in Hti;
+      cbn in Hti; destruct Hti as [[Hvi Hti] Heqs'].
+    apply composite_valid_transition_projection in Hnext;
+      cbn in Hnext; destruct Hnext as [[Hvj Htj] Heq_s'].
+    rewrite Heq_s', state_update_neq in Heqs' by done.
+    specialize (IHHs2 (state_update IM s j (s1 j))).
+    spec IHHs2.
+    {
+      split with (existT j lj) iom oom.
+      apply composite_valid_transition_projection_inv with (s1 j) (s' j).
+      - by split.
+      - apply state_update_eq.
+      - rewrite state_update_twice.
+        symmetry; apply state_update_id.
+        apply f_equal with (f := fun s => s j) in Heqs'.
+        by rewrite state_update_eq, state_update_neq in Heqs'.
+    }
+    cut (input_valid_transition RFree (existT i li) (state_update IM s j (s1 j), om) (s1, om')).
+    { by intros; eapply input_valid_transition_destination. }
+    repeat split; [done | apply any_message_is_valid_in_preloaded |..].
+    + by cbn; rewrite state_update_neq.
+    + cbn; rewrite state_update_neq by done.
+      replace (vtransition _ _ _) with (s' i, om').
+      f_equal; extensionality k; apply f_equal with (f := fun s => s k) in Heqs'.
+      destruct (decide (i = k)); [|destruct (decide (j = k))].
+      * by subst; rewrite state_update_eq, Heq_s', state_update_neq.
+      * by subst; rewrite state_update_neq, state_update_eq.
+      * by rewrite !state_update_neq in Heqs' |- *.
+Qed.
+
+Definition composite_valid_transitions_from_to : relation (composite_state IM) :=
+  tc CompositeValidTransitionNext.
+
+Lemma composite_valid_transitions_from_to_reflects_rechability :
+  forall s1 s2, composite_valid_transitions_from_to s1 s2 ->
+    valid_state_prop RFree s2 -> valid_state_prop RFree s1.
+Proof. by apply tc_reflect, CompositeValidTransitionNext_reflects_rechability. Qed.
+
+End sec_composite_succ.
